Move [cptrR] to a new file to break dependence on [wp].

theories/lang/cpp/logic/heap_pred.v
@@ -11,7 +11,7 @@ From iris_string_ident Require Import ltac2_string_ident.
 Require Import bedrock.prelude.base.
 
 From bedrock.lang.cpp Require Import
-     semantics ast logic.pred logic.path_pred logic.rep logic.wp.
+     semantics ast logic.pred logic.path_pred logic.rep.
 Export bedrock.lang.cpp.logic.rep.
 
 Implicit Types (σ resolve : genv) (p : ptr) (o : offset).
@@ -41,24 +41,7 @@ Section defs.
   Definition type_ptrR := type_ptrR_aux.(unseal).
   Definition type_ptrR_eq : @type_ptrR = _ := type_ptrR_aux.(seal_eq).
 
-  (* this is the core definition that the program logic will be based on.
-     it is really an assertion about assembly.
-   *)
-  Definition cptrR_def {resolve : genv} (fs : function_spec) : Rep :=
-    as_Rep (fun p =>
-         strict_valid_ptr p **
-         □ (Forall vs Q,
-         [| List.length vs = List.length fs.(fs_arguments) |] -*
-         fs.(fs_spec) vs Q -*
-         fspec resolve.(genv_tu).(globals) (type_of_spec fs) (Vptr p) vs Q)).
-  Definition cptrR_aux : seal (@cptrR_def). Proof. by eexists. Qed.
-  Definition cptrR := cptrR_aux.(unseal).
-  Definition cptrR_eq : @cptrR = _ := cptrR_aux.(seal_eq).
 End defs.
-
-#[global] Instance: Params (@cptrR) 3 := {}.
-
-Arguments cptrR {_ Σ resolve} _ : rename.
 
 Arguments type_ptrR {_ Σ σ} _%bs.
 Arguments identityR {_ Σ σ} _%bs _%bs _%Qp.
@@ -254,53 +237,6 @@ Section with_cpp.
   #[global] Instance anyR_observe_frac_valid resolve ty (q : Qp) :
     Observe [| q ≤ 1 |]%Qp (anyR ty q).
   Proof. rewrite anyR_eq. apply _. Qed.
-
-  #[global] Instance cptrR_persistent {resolve s} : Persistent (cptrR s).
-  Proof. rewrite cptrR_eq. apply _. Qed.
-  #[global] Instance cptrR_affine {resolve s} : Affine (cptrR s).
-  Proof. rewrite cptrR_eq. apply _. Qed.
-
-
-  Lemma cptrR_strict_valid_observe {resolve:genv} (p : ptr) f : Observe (strict_valid_ptr p) (_at p (cptrR f)).
-  Proof.
-    apply observe_intro_persistent; refine _.
-    rewrite cptrR_eq/cptrR_def _at_as_Rep.
-    iIntros "[$ _]".
-  Qed.
-
-  (* NOTE this should become an instance. *)
-  Lemma cptrR_valid_observe {resolve:genv} (p : ptr) f : Observe (valid_ptr p) (_at p (cptrR f)).
-  Proof. apply observe_strict_valid_valid; apply cptrR_strict_valid_observe. Qed.
-
-  Lemma cptrR_fs_impl {resolve} f g :
-    pureR (fs_impl f g) |-- cptrR f -* cptrR g.
-  Proof.
-    rewrite cptrR_eq/cptrR_def /pureR /as_Rep.
-    constructor => p; rewrite Rep_wand_force; iIntros "#(%ty & fs_impl)" => /=.
-    iIntros "(val & #rest)"; iFrame. iIntros (vs Q len).
-    rewrite ty. iModIntro. iIntros "fs_g".
-    iApply "rest"; first by apply length_type_of_spec in ty; rewrite -ty len.
-    by iApply "fs_impl".
-  Qed.
-
-(* TODO: Proper wrt [genv_leq]. *)
-  #[global] Instance cptrR_ne {resolve} : NonExpansive cptrR.
-  Proof.
-    intros n P Q HPQ. rewrite cptrR_eq. rewrite/cptrR_def.
-    rewrite (length_fs_arguments_ne _ _ _ HPQ) (type_of_spec_ne _ _ _ HPQ).
-    apply as_Rep_ne=>p. (do 2!f_equiv). do 6 f_equiv. by apply fs_spec_ne.
-  Qed.
-  #[global] Instance cptrR_proper {resolve} : Proper (equiv ==> equiv) cptrR.
-  Proof. exact: ne_proper. Qed.
-
-  #[global] Instance cptrR_mono {resolve} : Proper (fs_entails ==> (⊢)) cptrR.
-  Proof.
-    intros ??; rewrite /fs_entails/flip => impl. iApply cptrR_fs_impl.
-    by rewrite -impl pureR_emp.
-  Qed.
-
-  #[global] Instance cptrR_flip_mono {resolve} : Proper (flip fs_entails ==> flip (⊢)) cptrR.
-  Proof. by intros ?? <-. Qed.
 
 End with_cpp.
 
@@ -617,6 +553,3 @@ End with_cpp.
 
 Typeclasses Opaque identityR.
 Typeclasses Opaque type_ptrR validR svalidR alignedR.
-
-Instance Persistent_spec `{Σ:cpp_logic ti} {resolve:genv} nm s :
-  Persistent (_at (Σ:=Σ) (_global nm) (cptrR s)) := _.
