theories/lang/cpp/logic/cptr.v
@@ -1,0 +1,89 @@
+(*
+ * Copyright (c) 2021 BedRock Systems, Inc.
+ * This software is distributed under the terms of the BedRock Open-Source License.
+ * See the LICENSE-BedRock file in the repository root for details.
+ *)
+From iris.bi Require Export monpred.
+From iris.proofmode Require Import tactics monpred.
+From iris_string_ident Require Import ltac2_string_ident.
+
+Require Import bedrock.prelude.base.
+
+From bedrock.lang.cpp Require Import
+     semantics logic.pred logic.rep logic.wp.
+Export bedrock.lang.cpp.logic.rep.
+
+Section defs.
+  Context `{Σ : cpp_logic}.
+
+  (* this is the core definition that the program logic will be based on.
+     it is really an assertion about assembly.
+   *)
+  Definition cptrR_def {resolve : genv} (fs : function_spec) : Rep :=
+    as_Rep (fun p =>
+         strict_valid_ptr p **
+         □ (Forall vs Q,
+         [| List.length vs = List.length fs.(fs_arguments) |] -*
+         fs.(fs_spec) vs Q -*
+         fspec resolve.(genv_tu).(globals) (type_of_spec fs) (Vptr p) vs Q)).
+  Definition cptrR_aux : seal (@cptrR_def). Proof. by eexists. Qed.
+  Definition cptrR := cptrR_aux.(unseal).
+  Definition cptrR_eq : @cptrR = _ := cptrR_aux.(seal_eq).
+End defs.
+
+#[global] Instance: Params (@cptrR) 3 := {}.
+
+#[global] Arguments cptrR {_ Σ resolve} _ : rename.
+
+Section with_cpp.
+  Context `{Σ : cpp_logic} {resolve : genv}.
+
+  #[global] Instance cptrR_persistent {s} : Persistent (cptrR s).
+  Proof. rewrite cptrR_eq. apply _. Qed.
+  #[global] Instance cptrR_affine {s} : Affine (cptrR s).
+  Proof. rewrite cptrR_eq. apply _. Qed.
+
+  Lemma cptrR_strict_valid_observe (p : ptr) f : Observe (strict_valid_ptr p) (_at p (cptrR f)).
+  Proof.
+    apply observe_intro_persistent; refine _.
+    rewrite cptrR_eq/cptrR_def _at_as_Rep.
+    iIntros "[$ _]".
+  Qed.
+
+  (* NOTE this should become an instance. *)
+  Lemma cptrR_valid_observe (p : ptr) f : Observe (valid_ptr p) (_at p (cptrR f)).
+  Proof. apply observe_strict_valid_valid; apply cptrR_strict_valid_observe. Qed.
+
+  Lemma cptrR_fs_impl f g :
+    pureR (fs_impl f g) |-- cptrR f -* cptrR g.
+  Proof.
+    rewrite cptrR_eq/cptrR_def /pureR /as_Rep.
+    constructor => p; rewrite Rep_wand_force; iIntros "#(%ty & fs_impl)" => /=.
+    iIntros "(val & #rest)"; iFrame. iIntros (vs Q len).
+    rewrite ty. iModIntro. iIntros "fs_g".
+    iApply "rest"; first by apply length_type_of_spec in ty; rewrite -ty len.
+    by iApply "fs_impl".
+  Qed.
+
+(* TODO: Proper wrt [genv_leq]. *)
+  #[global] Instance cptrR_ne : NonExpansive cptrR.
+  Proof.
+    intros n P Q HPQ. rewrite cptrR_eq. rewrite/cptrR_def.
+    rewrite (length_fs_arguments_ne _ _ _ HPQ) (type_of_spec_ne _ _ _ HPQ).
+    apply as_Rep_ne=>p. (do 2!f_equiv). do 6 f_equiv. by apply fs_spec_ne.
+  Qed.
+  #[global] Instance cptrR_proper : Proper (equiv ==> equiv) cptrR.
+  Proof. exact: ne_proper. Qed.
+
+  #[global] Instance cptrR_mono : Proper (fs_entails ==> (⊢)) cptrR.
+  Proof.
+    intros ??; rewrite /fs_entails/flip => impl. iApply cptrR_fs_impl.
+    by rewrite -impl pureR_emp.
+  Qed.
+
+  #[global] Instance cptrR_flip_mono : Proper (flip fs_entails ==> flip (⊢)) cptrR.
+  Proof. by intros ?? <-. Qed.
+End with_cpp.
+
+#[global] Instance Persistent_spec `{Σ:cpp_logic ti} {resolve:genv} p s :
+  Persistent (_at (Σ:=Σ) p (cptrR s)) := _.
